theories/tree_borrows/step_laws/steps_prot.v
@@ -9,7 +9,7 @@ From simuliris.tree_borrows Require Import steps_progress steps_inv.
 From simuliris.tree_borrows Require Import logical_state inv_accessors.
 From simuliris.tree_borrows Require Import wishlist.
 From simuliris.tree_borrows.trees_equal Require Import trees_equal_base random_lemmas.
-From simuliris.tree_borrows.trees_equal Require Import trees_equal_asymmetric_read trees_equal_transitivity.
+From simuliris.tree_borrows.trees_equal Require Import trees_equal_asymmetric_prot trees_equal_transitivity.
 From iris.prelude Require Import options.
 
 (** * Simulation lemmas using the ghost state for proving optimizations *)
