theories/tree_borrows/trees_equal/trees_equal_source_read.v
@@ -1,0 +1,180 @@
+(** This file provides the basic heap and ghost state support for the BorIngLang program logic. *)
+From iris.proofmode Require Export proofmode.
+From iris.bi.lib Require Import fractional.
+From iris.base_logic.lib Require Import ghost_map.
+From simuliris.base_logic Require Export gen_sim_prog.
+From simuliris.simulation Require Export slsls gen_log_rel.
+From simuliris.simulation Require Import lifting.
+From simuliris.tree_borrows Require Import tkmap_view.
+From simuliris.tree_borrows Require Export defs.
+From simuliris.tree_borrows Require Export steps_wf.
+From simuliris.tree_borrows Require Import steps_progress.
+From simuliris.tree_borrows.trees_equal Require Import trees_equal_base random_lemmas.
+From iris.prelude Require Import options.
+
+(* TODO cleanup *)
+Section utils.
+
+Context (C : call_id_set).
+
+  (* Remember that the entire reason we have [trees_equal] in the first place
+     is to enable spurious reads. This is the lemma that verifies that after we
+     do a spurious read we get a [tree_equal].
+     Specifically, it is for source-only spurious reads.
+     This means we do not need to prove they succeed, we _get_ this as an assumption.
+     All that is necessary in addition is showing that equality is preserved.
+
+     The resulting direction is backwards because we later use the transitivity that has
+       new_source =Forwards= old_source =Forwards= old_target,
+     but the lemma is stated as old_source =Backwards= new_source for mostly historical reasons
+     and laziness.
+   *)
+  Lemma tree_equal_asymmetric_read_source
+    {tr tr' acc_tg range it} (mode:bool)
+    (GloballyUnique : forall tg, tree_contains tg tr -> tree_unique tg tr)
+    :
+    (* Accessed tag must be in the tree and protected*)
+    tree_lookup tr acc_tg it ->
+    tree_equal_asymmetric_read_pre_source tr range it acc_tg mode ->
+    (* Under the above conditions if we do a spurious read and it succeeds
+       we get a [tree_equal] on the outcome. *)
+    memory_access AccessRead C acc_tg range tr = Some tr' ->
+    tree_equal C Backwards tr tr'.
+  Proof.
+    intros Lkup TreeShapeProper Acc.
+    split; last split.
+    { intro tg. eapply access_preserves_tags. eassumption. }
+    { intros tg1 tg2. eapply access_same_rel_dec. eassumption. }
+    (* That was the easy part, helped by the fact that our initial configuration
+       is reflexivity instead of a more general instance of [tree_equal].
+       Soon it will get more interesting. *)
+    intros tg0 Ex.
+    destruct (unique_implies_lookup (GloballyUnique _ Ex)) as [it0 Lookup0].
+    exists it0.
+    assert (tree_unique tg0 tr') as Unq0'. {
+      erewrite <- tree_apply_access_preserve_unique; last eassumption.
+      apply GloballyUnique. assumption.
+    }
+    destruct (apply_access_spec_per_node (proj1 Lookup0) (proj2 Lookup0) Acc) as
+        (it0' & it0'Spec & Ex0' & Det0').
+    symmetry in it0'Spec.
+    exists it0'.
+    split; first assumption.
+    split; first (split; assumption).
+    (* Now down to per-item reasoning *)
+    intro loc.
+    split; first (eapply item_apply_access_preserves_metadata; eassumption).
+    rewrite bind_Some in it0'Spec; destruct it0'Spec as (perms' & perms'Spec & [= <-]).
+    pose proof (mem_apply_range'_spec _ _ loc _ _ perms'Spec) as PerLoc.
+    clear perms'Spec.
+    assert (itag it0 = tg0) by (eapply tree_determined_specifies_tag; eapply Lookup0).
+    assert (itag it = acc_tg) by (eapply tree_determined_specifies_tag; eapply Lkup).
+    subst.
+    (* Finally the reasoning is per-location *)
+    destruct (decide _) as [HinRange|?]; last first.
+    { rewrite /item_lookup /= PerLoc.
+      constructor. }
+    destruct (TreeShapeProper _ HinRange) as (Htginit&Htgnondis&Hothers).
+    (* Keep digging until [apply_access_perm_inner] *)
+    destruct PerLoc as (perm' & perm'Lookup & perm'Spec).
+    pose proof Hothers as Hothers_pure.
+    ospecialize (Hothers _ _ Lookup0).
+    change (default _ _) with (item_lookup it0 loc) in perm'Spec.
+    rewrite {2}/item_lookup perm'Lookup /=.
+    rewrite bind_Some in perm'Spec; destruct perm'Spec as (tmperm & Inner & perm'Spec).
+    rewrite bind_Some in perm'Spec; destruct perm'Spec as (validated & MoreInit & EqPerm).
+    injection EqPerm; clear EqPerm; intros; subst.
+    rewrite rel_dec_flip2 in Hothers.
+    destruct Hothers as (Hothers&Hspecials).
+    destruct (rel_dec tr (itag it) (itag it0)) as [[]|[]] eqn:Hreldec.
+    - destruct mode.
+      + assert (∃ tg, tree_contains tg tr ∧ rel_dec tr tg (itag it) = Child (Strict Immediate) ∧ ParentChildIn tg (itag it0) tr) as (tgsw & Hin & Hswdec&Hpar).
+        { rewrite /rel_dec in Hreldec. destruct decide as [HP|HnP]; try done. destruct decide as [HP|?]; try done.
+          destruct HP as [Heq|HSP]. 1: exfalso; eapply HnP; by left.
+          eapply immediate_sandwich in HSP as HSP2. 2, 3: eapply GloballyUnique. 2: eapply Lkup.
+          destruct HSP2 as (tsw&Htsw&HPC). exists tsw.
+          assert (tree_contains tsw tr) as Hcont.
+          { eapply contains_child. 1: right; by eapply Immediate_is_StrictParentChild.
+            eapply Lkup. }
+           split_and!. 1: done. 2: done.
+          rewrite /rel_dec decide_True. 
+          2: right; by eapply Immediate_is_StrictParentChild.
+          rewrite decide_False. 1: by rewrite decide_True.
+          intros HH. eapply immediate_parent_not_child. 4: exact HH. 3: done.
+          all: eapply GloballyUnique. 1: eapply Lkup. done. }
+        assert (∃ itsw, tree_lookup tr tgsw itsw) as (itsw&Hitsw).
+        1: eapply unique_implies_lookup, GloballyUnique, Hin.
+        specialize (Hothers_pure _ _ Hitsw).
+        destruct (apply_access_spec_per_node (proj1 Hitsw) (proj2 Hitsw) Acc) as
+        (itsw' & itsw'Spec & Hitsw').
+        destruct Hothers_pure as (_&HH). ospecialize (HH _). 1: done.
+        eapply (perm_eq_up_to_C_disabled_parent C _ _ _ _ _ _ tgsw). 3: rewrite /= most_init_comm //=.
+        * econstructor. 2: done. 1: rewrite /rel_dec decide_True //.
+          destruct (item_lookup itsw loc) as [[] pp] eqn:HHH; simpl in *; subst pp.
+          1: econstructor 1. econstructor 2. econstructor 1.
+        * econstructor. 1: erewrite <- access_same_rel_dec. 2: eassumption. 1: rewrite /rel_dec decide_True //.
+          1: exact Hitsw'. symmetry in itsw'Spec.
+          eapply bind_Some in itsw'Spec as (psw&Hsw&[= Hitsweq]).
+          pose proof (mem_apply_range'_spec _ _ loc _ _ Hsw) as PerLocSW.
+          rewrite decide_True // in PerLocSW. destruct PerLocSW as (p & HPP & Hacc).
+          rewrite /= /apply_access_perm /apply_access_perm_inner /= in Hacc.
+          change (default _ _) with (item_lookup itsw loc) in Hacc.
+          assert (itag itsw = tgsw) as <- by by eapply tree_lookup_correct_tag.
+          rewrite rel_dec_flip2 Hswdec /= HH /= most_init_comm /= in Hacc.
+          rewrite /item_lookup /= -Hitsweq HPP /=.
+          destruct (item_lookup itsw loc) as [ini prm] eqn:Heq; simpl in *; subst prm.
+          edestruct (bool_decide (protector_is_active (iprot itsw) C)), ini in Hacc; simpl in Hacc; try discriminate Hacc; injection Hacc as <-.
+          all: try econstructor 1. all: econstructor 2; econstructor 1.
+      + rewrite /apply_access_perm_inner /= in Inner. rewrite /= most_init_comm /=.
+        destruct Hspecials as (Hfrz&Hnact).
+        destruct (item_lookup it0 loc) as [ini [cfl| | | |]] eqn:Hperm.
+        2,4,5: by (destruct ini, (bool_decide (protector_is_active (iprot it0) C)); simpl in *; simplify_eq; econstructor 1).
+        2: exfalso; by eapply Hnact.
+        simpl in *. assert (∃ cfl', validated = Reserved cfl') as (cfl'&->).
+        { destruct ini, cfl, (bool_decide (protector_is_active (iprot it0) C)); simpl in *; eexists; simplify_eq; done. }
+        destruct (apply_access_spec_per_node (proj1 Lkup) (proj2 Lkup) Acc) as
+        (it' & it'Spec & Hit'). symmetry in it'Spec.
+        eapply bind_Some in it'Spec as (pit&Hpit&[= Hiteq]).
+        pose proof (mem_apply_range'_spec _ _ loc _ _ Hpit) as PerLoc.
+        rewrite decide_True // in PerLoc. destruct PerLoc as (p & HPP & Hacc).
+        rewrite /= /apply_access_perm /apply_access_perm_inner /= in Hacc.
+        change (default _ _) with (item_lookup it loc) in Hacc.
+        assert (itag it' = itag it) as Hit by by eapply tree_lookup_correct_tag.
+        rewrite rel_dec_refl Hfrz /= most_init_comm /= in Hacc.
+        rewrite Tauto.if_same /= in Hacc. injection Hacc as <-.
+        eapply perm_eq_up_to_C_frozen_parent with (witness_tg := itag it).
+        econstructor.
+        { erewrite <- access_same_rel_dec. 2: done. rewrite rel_dec_flip2 Hreldec //. }
+        { eapply Hit'. }
+        all: rewrite /item_lookup -Hiteq /= HPP /= //.
+    - rewrite /= most_init_comm /=.
+      rewrite /apply_access_perm_inner /= in Inner.
+      destruct (item_lookup it0 loc) as [[] [[]| | | |]] eqn:Hperm, (bool_decide (protector_is_active (iprot it0) C)) eqn:Hprot; simpl in *.
+      all: try by (simplify_eq; econstructor 1).
+      all: simplify_eq.
+      all: destruct (decide (protector_is_active (iprot it0) C)) as [HProt|HNoProt];
+             first (econstructor 7; econstructor; done).
+      all: by econstructor 3.
+    - destruct Hothers as (Hinit&Hndis).
+      rewrite /apply_access_perm_inner /= in Inner.
+      destruct (item_lookup it0 loc) as [[] pp] eqn:Hperm. 2: done.
+      assert (pp = tmperm) as ->.
+      { simpl in *. destruct pp; simplify_eq; done. }
+      rewrite /= in MoreInit|-*.
+      destruct tmperm, (bool_decide (protector_is_active (iprot it0) C)); simpl in MoreInit.
+      all: try done. all: simplify_eq; econstructor 1.
+    - simpl in *. assert (itag it = itag it0) as Htageq.
+      { rewrite /rel_dec in Hreldec. do 2 (destruct decide; try done).
+        eapply mutual_parent_child_implies_equal. 1: done. 1: eapply Lkup. all: done. }
+      assert (it = it0) as ->.
+      { eapply tree_determined_unify. 1, 2: eapply Lkup. rewrite Htageq. eapply Lookup0. }
+      rewrite Htginit /= in MoreInit|-*.
+      assert (tmperm = validated) as ->.
+      { destruct bool_decide in MoreInit; last by congruence.
+        destruct tmperm; congruence. }
+      clear MoreInit.
+      destruct (item_lookup it0 loc) as [[] pp] eqn:Hperm. 2: done.
+      destruct pp; try done. all: repeat (simpl in *; simplify_eq); by econstructor 1.
+  Qed.
+
+End utils.
